src/FcEtt/ext_weak.v
@@ -1,11 +1,10 @@
+
 Require Import FcEtt.tactics.
 Require Import FcEtt.utils.
 Require Export FcEtt.imports.
-
 Require Export FcEtt.ett_inf.
 (* Require Export FcEtt.ett_par. *)
 Require Export FcEtt.ett_ind.
-
 Require Import FcEtt.ext_wf.
 
 Set Bullet Behavior "Strict Subproofs".
@@ -137,9 +136,8 @@ Proof.
   unfold not.
   intros b. destruct b as [phi b].
   assert (Tm A' R' = Co phi). eapply binds_unique; eauto.
-  by eauto using wf.DefEq_Ctx, wf.Ctx_uniq.
-  inversion H2.
-  fsetdec.
+  by eauto using DefEq_Ctx, Ctx_uniq. symmetry.
+  auto.
 Qed.
 
 (* ----- *)
