src/FcEtt/fc_subst.v
@@ -1,3 +1,5 @@
+Require Import FcEtt.sigs.
+
 Require Import FcEtt.tactics.
 
 Require Export FcEtt.imports.
@@ -17,6 +19,11 @@ Require Export FcEtt.fc_wf.
 Require Export FcEtt.fc_context_fv.
 
 Import FcEtt.ett_ott.
+
+Module fc_subst (wf : fc_wf_sig) (weak : fc_weak_sig) <: fc_subst_sig.
+
+Export wf.
+Export weak.
 
 Set Bullet Behavior "Strict Subproofs".
 Set Implicit Arguments.
@@ -1549,3 +1556,5 @@ Proof.
     rewrite (co_subst_co_co_fresh_eq); auto.
     eauto.
 Qed.
+
+End fc_subst.
